src/impl/TLS13.Impl.Driver.PairingNoTailRawBridge.fsti
@@ -242,7 +242,6 @@ val lemma_equal_stream_head_received_server_hello_not_change_cipher_spec
   (ccs_tail:B.bytes)
   : Lemma
       (requires
-        WFL.supported_server_hello_wire_profile sh /\
         Seq.equal left_stream right_stream /\
         Seq.equal left_stream (B.append server_hello_raw server_tail) /\
         Seq.equal right_stream (B.append ccs_raw ccs_tail) /\
@@ -829,8 +828,6 @@ val lemma_normalized_cleartext_raw_wire_bridge_from_role_local_prefixes
           server_sh
           server_rest /\
         WFL.supported_client_hello_wire_profile client_ch /\
-        WFL.supported_server_hello_wire_profile server_sh /\
-        WFL.supported_server_hello_wire_profile client_sh /\
         CS.connection_state_raw_event_replay_consistent client /\
         CS.connection_state_raw_event_replay_consistent server /\
         CS.paired_wire_logs client server)
